(a) When we multiply
\[
\frac{1}{(1 - 2x)(3x - 1)} = \frac{A}{1 - 2x} + \frac{B}{3x - 1} \tag{1}
\]
with $(1 - 2x)(3x - 1)$, we get
\[
1 = ??? \tag{2}
\]

Substituting $x = ???$ into (2), we get
\begin{align*}
                 ??? &= ??? \\
\THEREFORE  \,\,\, A &= ??? \tag{3} 
\end{align*}
Substituting $x = ???$ into (2), we get
\begin{align*}
                  ??? &= ??? \\
\THEREFORE \,\,\, B   &= ??? \tag{4} 
\end{align*}

ANSWER:
\boxed{A=???, \hspace{1cm} B=???}
\qed


(b)
Substituting (3) and (4) into (1) we get
\begin{align*}
f(x) 
&= \frac{1}{(1 - 2x)(3x - 1)} 
\\
&= ??? \frac{1}{1 - 2x} + ??? \frac{1}{3x - 1} 
\\
&= ??? 
\\
&= ??? 
\\
&= ??? 
\\
\end{align*}

ANSWER:
\boxed{???}
\qed

(c)

ANSWER:
\boxed{???}
\qed
